demo

demo/Fibo32.fst
@@ -16,54 +16,51 @@
 
 module Fibo32
 #lang-pulse
-open Pulse.Lib.Pervasives
-module U32 = FStar.UInt32
-#push-options "--fuel 2 --ifuel 2"
-
 
 let rec fib (n:nat) : nat =
   if n <= 1 then 1
   else fib (n - 1) + fib (n - 2)
 
-let rec fib_mono (n:nat) (m:nat { m <= n})
+open Pulse.Lib.Pervasives
+module U32 = FStar.UInt32
+open Pulse.Lib.BoundedIntegers
+
+let rec fib_mono (n:nat) (m:nat {m <= n})
   : Lemma
     (ensures fib m <= fib n)
   = if n = m then ()
     else fib_mono (n - 1) m
 
-open Pulse.Lib.BoundedIntegers
 
-#push-options "--z3rlimit_factor 4"
-
-fn fibo32 (k:U32.t) (_:squash(0ul < k /\ fits #U32.t (fib (v k))))
-  requires emp
-  returns r:U32.t
-  ensures pure (v r == fib (v k))
+fn fibo32 (k:U32.t)
+  requires
+    pure (k > 0ul /\ fits #U32.t (fib (v k)))
+  returns
+    r : U32.t
+  ensures
+    pure (v r == fib (v k))
 {
   let mut i = 1ul;
   let mut j = 1ul;
   let mut ctr = 1ul;
   while (let vctr = !ctr; (vctr < k))
-  invariant b . exists* vi vj vctr. (
+    invariant b. exists* vi vj vctr.
      pts_to i vi **
      pts_to j vj **
-     pts_to ctr vctr **     
+     pts_to ctr vctr **
      pure (1ul <= vctr /\
            vctr <= k /\
-           fib (v vctr - 1) == v vi/\
-           fib (v vctr) == v vj /\
+           fib (v vctr - 1) == v vi /\ fib (v vctr) == v vj /\
            b == (vctr < k))
-  )
   {
      let vc = !ctr;
      let vi = !i;
      let vj = !j;
      ctr := vc + 1ul;
      i := vj;
-    //  fib_mono (v k) (v vc + 1);
+     fib_mono (v k) (v vc + 1);
      j := vi + vj;
      ()
   };
-  let r = !j;
-  r
+  !j;
 }
